Use bitwise equality for equality of module outputs
Allows the solver to solve each output bit individually, which is
faster for certain designs designs (like AddMulUns).

vera/VerilogEquivalence.v
@@ -38,6 +38,8 @@ Import FunctorNotation.
 Local Open Scope monad_scope.
 Local Open Scope string.
 
+Opaque N.le N.of_nat N.to_nat.
+
 Definition mk_var_same (var : Var.t) : (SMTLib.term SMTLib.Sort_Bool) := 
   SMTLib.Term_Eq (SMTLib.Term_Const (verilog_to_smt_var VerilogLeft var))
                  (SMTLib.Term_Const (verilog_to_smt_var VerilogRight var)).
@@ -47,10 +49,31 @@ Equations mk_inputs_same (inputs : list Var.t) : SMTLib.term SMTLib.Sort_Bool :=
   | (var :: vars) => SMTLib.Term_And (mk_var_same var) (mk_inputs_same vars)
 }.
 
+Section eq_bitwise.
+  Variable (w : N) (t1 t2 : SMTLib.term (SMTLib.Sort_BitVec w)).
+
+  Equations eq_bitwise (idx : nat) (wf : (N.of_nat idx <= w)%N) : SMTLib.term SMTLib.Sort_Bool := {
+    | 0, wf => SMTLib.Term_True
+    | S idx_pred, wf =>
+      let idx := N.of_nat idx_pred in
+      SMTLib.Term_And
+        (SMTLib.Term_Eq (SMTLib.Term_BVExtract idx idx (reflexivity idx) t1) (SMTLib.Term_BVExtract idx idx (reflexivity idx) t2))
+        (eq_bitwise idx_pred _)
+  }.
+  Next Obligation. lia. Qed. 
+End eq_bitwise.
+
+(* Definition mk_var_distinct (var : Var.t) : SMTLib.term SMTLib.Sort_Bool :=
+ *   SMTLib.Term_Not (SMTLib.Term_Eq (SMTLib.Term_Const (verilog_to_smt_var VerilogLeft var))
+ *                                   (SMTLib.Term_Const (verilog_to_smt_var VerilogRight var)))
+ *   . *)
+#[program]
 Definition mk_var_distinct (var : Var.t) : SMTLib.term SMTLib.Sort_Bool :=
-  SMTLib.Term_Not (SMTLib.Term_Eq (SMTLib.Term_Const (verilog_to_smt_var VerilogLeft var))
-                                  (SMTLib.Term_Const (verilog_to_smt_var VerilogRight var)))
+  SMTLib.Term_Not (eq_bitwise _ (SMTLib.Term_Const (verilog_to_smt_var VerilogLeft var))
+                                (SMTLib.Term_Const (verilog_to_smt_var VerilogRight var))
+                                (N.to_nat (Var.varType var)) _)
   .
+Next Obligation. lia. Qed.
 
 Equations mk_outputs_distinct (inputs : list Var.t) : SMTLib.term SMTLib.Sort_Bool := {
   | [] => SMTLib.Term_False
